First sketch of automation

src/num/theories/cv_compute/automation/cv_typesScript.sml
@@ -104,15 +104,12 @@ QED
 
 Definition from_option_def:
   from_option f NONE = Num 0 /\
-  from_option f (SOME x) =
-    case f x of
-    | Num n => Num (n+1)
-    | other => other
+  from_option f (SOME x) = Pair (Num 1) (f x)
 End
 
 Definition to_option_def:
-  to_option t (Num n) = (if n = 0 then NONE else SOME (t (Num (n - 1)))) /\
-  to_option t other = SOME (t other)
+  to_option t (Num n) = NONE /\
+  to_option t (Pair x y) = if x = Num 1 then SOME (t y) else NONE
 End
 
 Theorem from_to_option:
@@ -120,27 +117,26 @@ Theorem from_to_option:
   from_to (from_option f) (to_option t)
 Proof
   fs [from_to_def] \\ strip_tac
-  \\ Cases \\ fs [from_option_def]
-  \\ Cases_on ‘f x'’ \\ fs [to_option_def]
-  \\ pop_assum $ assume_tac o GSYM \\ fs []
+  \\ Cases \\ fs [from_option_def,to_option_def]
 QED
 
 (* pair *)
 
-Definition from_prod_def:
-  from_prod f1 f2 (x,y) = Pair (f1 x) (f2 y)
+Definition from_pair_def:
+  from_pair f1 f2 (x,y) = Pair (f1 x) (f2 y)
 End
 
-Definition to_prod_def:
-  to_prod t1 t2 (Pair x y) = (t1 x, t2 y)
+Definition to_pair_def:
+  to_pair t1 t2 (Pair x y) = (t1 x, t2 y) /\
+  to_pair t1 t2 _ = ARB
 End
 
-Theorem from_to_prod:
+Theorem from_to_pair:
   from_to f1 t1 /\ from_to f2 t2 ==>
-  from_to (from_prod f1 f2) (to_prod t1 t2)
+  from_to (from_pair f1 f2) (to_pair t1 t2)
 Proof
   fs [from_to_def] \\ strip_tac
-  \\ Cases \\ fs [from_prod_def,to_prod_def]
+  \\ Cases \\ fs [from_pair_def,to_pair_def]
 QED
 
 (* sum *)
@@ -151,8 +147,10 @@ Definition from_sum_def:
 End
 
 Definition to_sum_def:
+  to_sum t1 t2 (Num n) = ARB /\
   to_sum t1 t2 (Pair x y) =
-    if x = Num 0 then INL (t1 y) else INR (t2 y)
+    if x = Num 0 then INL (t1 y) else
+    if x = Num 1 then INR (t2 y) else ARB
 End
 
 Theorem from_to_sum:
@@ -182,5 +180,473 @@ Proof
   fs [from_to_def] \\ strip_tac
   \\ Induct \\ fs [from_list_def,to_list_def]
 QED
+
+(* used in definitions of to-functions of user-defined datatype *)
+
+Definition cv_has_shape_def:
+  cv_has_shape (SOME n::xs) (Pair x y) = (x = Num n /\ cv_has_shape xs y) /\
+  cv_has_shape (NONE::xs) (Pair x y) = cv_has_shape xs y /\
+  cv_has_shape (_::xs) (Num _) = F /\
+  cv_has_shape [] c = T
+End
+
+Theorem cv_has_shape_expand:
+  cv_has_shape [] cv = T /\
+  cv_has_shape (NONE::xs) cv = (?x y. cv = Pair x y /\ cv_has_shape xs y) /\
+  cv_has_shape (SOME n::xs) cv = (?y. cv = Pair (Num n) y /\ cv_has_shape xs y)
+Proof
+  Cases_on ‘cv’ \\ fs [cv_has_shape_def]
+QED
+
+(* lemmas for automation *)
+
+Theorem get_to_pair:
+  (if cv_has_shape [NONE] v then (t1 (cv_fst v),t2 (cv_snd v)) else ARB) =
+  to_pair t1 t2 v
+Proof
+  Cases_on ‘v’
+  \\ fs [to_pair_def,cv_has_shape_def]
+QED
+
+Theorem get_to_option:
+  (if cv_has_shape [SOME 1] v then SOME (t (cv_snd v)) else NONE) = to_option t v
+Proof
+  Cases_on ‘v’
+  \\ fs [to_option_def,cv_has_shape_def]
+QED
+
+Theorem get_to_sum:
+  (if cv_has_shape [SOME 0] v then INL (t1 (cv_snd v))
+   else if cv_has_shape [SOME 1] v then INR (t2 (cv_snd v))
+   else ARB) = to_sum t1 t2 v
+Proof
+  Cases_on ‘v’
+  \\ fs [to_sum_def,cv_has_shape_def]
+QED
+
+Theorem get_from_sum:
+  (case v of INL x => Pair (Num 0) (f0 x) | INR y => Pair (Num 1) (f1 y)) =
+  from_sum f0 f1 v
+Proof
+  Cases_on ‘v’ \\ fs [from_sum_def]
+QED
+
+Theorem get_from_option:
+  (case v of NONE => Num 0 | SOME x => Pair (Num 1) (f x)) =
+  from_option f v
+Proof
+  Cases_on ‘v’ \\ fs [from_option_def]
+QED
+
+Theorem get_from_pair:
+  (case v of (v0,v1) => Pair (f0 v0) (f1 v1)) =
+  from_pair f0 f1 v
+Proof
+  Cases_on ‘v’ \\ fs [from_pair_def]
+QED
+
+(* ------------- automation ---------------- *)
+
+val ERR = mk_HOL_ERR "cv_typesLib";
+
+fun type_of_cases_const ty = let
+  val th = TypeBase.case_def_of ty
+  val ty = th |> SPEC_ALL |> CONJUNCTS |> hd |> SPEC_ALL
+              |> concl |> dest_eq |> fst |> repeat rator |> type_of
+  in ty end
+
+fun auto_prove proof_name (goal,tac:tactic) = let
+  val (rest,validation) = tac ([],goal)
+    handle HOL_ERR r => raise (ERR "auto_prove" "tactic failure")
+      | Empty => raise (ERR "auto_prove" "tactic raised Empty")
+  in if length rest = 0 then validation [] else let
+  in failwith("auto_prove failed for " ^ proof_name) end end
+
+fun dest_fun_type ty = let
+  val (name,args) = dest_type ty
+  in if name = "fun" then (el 1 args, el 2 args) else failwith("not fun type") end;
+
+fun find_mutrec_types ty = let (* e.g. input ``:v`` gives [``:exp``,``:v``]  *)
+  fun is_pair_ty ty = fst (dest_type ty) = "prod"
+  val xs = TypeBase.axiom_of ty
+           |> SPEC_ALL |> concl |> strip_exists
+           |> #1 |> map (#1 o dest_fun_type o type_of)
+           |> (fn ls => filter (fn ty => intersect ((#2 o dest_type) ty) ls = []) ls)
+  in if is_pair_ty ty then [ty] else if length xs = 0 then [ty] else xs end
+
+fun matching_induction_of typ = let
+    val ind = TypeBase.induction_of typ
+    val ind_c = concl ind |> strip_forall |> snd |> dest_imp |> snd
+    val var_tys = strip_conj ind_c |> map (type_of o fst o dest_forall)
+    val matches = mapfilter (fn vty => match_type vty typ) var_tys
+  in case matches of
+      [] => failwith ("matching_induction_of: " ^ type_to_string typ)
+    | _ => INST_TYPE (hd matches) ind
+  end
+
+fun mk_funtype arg_tys ret_ty =
+  if null arg_tys then ret_ty else
+    mk_funtype (butlast arg_tys) (mk_type("fun",[last arg_tys,ret_ty]));
+
+fun make_stem fname args ret_ty = let
+  val f_ty = mk_funtype (map type_of args) ret_ty
+  in list_mk_comb(mk_var(fname,f_ty),args) end
+
+fun alookup x [] = NONE
+  | alookup x ((y,z)::xs) = if x = y then SOME z else alookup x xs;
+
+fun dest_fun_types ty =
+  let
+    val (x,y) = dest_fun_type ty
+    val (xs,z) = dest_fun_types y
+  in
+    (x::xs,z)
+  end handle HOL_ERR _ => ([],ty);
+
+local
+  val sum_case = sumTheory.sum_case_def
+    |> CONJUNCTS |> hd |> SPEC_ALL |> concl |> dest_eq |> fst |> repeat rator
+  val tys = dest_fun_types (type_of sum_case) |> fst
+  val pat_args = mapi (fn i => fn ty => mk_var("v" ^ int_to_string i, ty)) tys
+  val pat = list_mk_comb(sum_case,pat_args)
+  val thm = REFL pat |> GENL pat_args
+in
+  fun mk_sum_case x y z = ISPECL [x,y,z] thm |> concl |> rand
+end
+
+fun mk_sum_type l_ty r_ty =
+  mk_thy_type {Args = [l_ty, r_ty], Thy = "sum", Tyop = "sum"};
+
+fun mk_pairs [] = cvSyntax.mk_cv_num(numSyntax.term_of_int 0)
+  | mk_pairs [x] = x
+  | mk_pairs (x::xs) = cvSyntax.mk_cv_pair(x, mk_pairs xs);
+
+fun constructors_of ty = let
+  val conses = TypeBase.constructors_of ty
+  fun match_ret_type c =
+    inst (match_type (repeat (snd o dest_fun_type) (type_of c)) ty) c
+  in map match_ret_type conses end
+
+fun from_to_for ty =
+  if ty = “:unit” then from_to_unit else
+  if ty = “:bool” then from_to_bool else
+  if ty = “:num” then from_to_num else
+  if ty = “:int” then from_to_int else
+  if listSyntax.is_list_type ty then
+    let val a = from_to_for (listSyntax.dest_list_type ty)
+    in MATCH_MP from_to_list a end
+  else fail()
+
+fun from_for ty = from_to_for ty |> concl |> rator |> rand;
+fun to_for ty = from_to_for ty |> concl |> rand;
+
+val num_ty = arithmeticTheory.ODD_EVEN |> concl |> dest_forall |> fst |> type_of
+val cv_has_shape_tm =
+  cv_has_shape_def |> CONJUNCT1 |> SPEC_ALL |> concl |> dest_eq |> fst |> repeat rator;
+
+fun replicate 0 x = []
+  | replicate n x = x :: replicate (n-1) x;
+
+(*
+val ty = “:('d, 'c) b”
+*)
+fun define_from_to ty = let
+  (* extract target structure from induction theorem *)
+  val mutrec_count = length (find_mutrec_types ty)
+  val ind = TypeBase.induction_of ty
+  val inputs = ind |> SPEC_ALL |> UNDISCH_ALL |> CONJUNCTS |> map (fst o dest_forall o concl)
+  val tyvars = dest_type (type_of (hd inputs)) |> snd
+  val first_name = inputs |> hd |> type_of |> dest_type |> fst
+  val names = inputs |> mapi (fn i => fn v =>
+    if i < mutrec_count then
+      ((v |> type_of |> dest_type |> fst), type_of v)
+    else
+      (first_name ^ int_to_string (i - mutrec_count + 1), type_of v))
+  (* define encoding into cv type, i.e. "from function" *)
+  val tyvar_encoders = mapi (fn i => fn ty =>
+    mk_var("f" ^ int_to_string i,mk_type("fun",[ty,cvSyntax.cv]))) tyvars
+  val from_names = names |>
+    map (fn (fname,ty) =>
+      make_stem ("from_" ^ fname) tyvar_encoders (mk_funtype [ty] cvSyntax.cv))
+  val lookups =
+    map (fn tm => (tm |> type_of |> dest_fun_type |> fst, tm)) (from_names @ tyvar_encoders)
+  (*
+  val from_f = el 4 from_names
+  *)
+  fun from_lines from_f = let
+    val conses = from_f |> type_of |> dest_type |> snd |> hd |> constructors_of
+    (*
+      val i = 0
+      val cons_tm = el 2 conses
+    *)
+    fun from_line i cons_tm = let
+      val (tys,target_ty) = dest_fun_types (type_of cons_tm)
+      val pat_args = mapi (fn i => fn ty => mk_var("v" ^ int_to_string i, ty)) tys
+      val pat = list_mk_comb(cons_tm,pat_args)
+      val lhs_tm = mk_comb(from_f,pat)
+      val tag_num = cvSyntax.mk_cv_num(numSyntax.term_of_int i)
+      fun process_arg v =
+        case alookup (type_of v) lookups of
+          SOME tm => mk_comb(tm,v)
+        | NONE => mk_comb(from_for (type_of v),v)
+      val args = map process_arg pat_args
+      val smart_mk_pairs =
+        (if listSyntax.is_cons pat then mk_pairs o tl else
+         if pairSyntax.is_pair pat then mk_pairs o tl else
+           mk_pairs)
+      val rhs_tm = smart_mk_pairs (tag_num :: args)
+      in mk_eq(lhs_tm,rhs_tm) end
+    val lines = mapi from_line conses
+    in lines end
+  val all_lines = map from_lines from_names |> flatten
+  val tm = list_mk_conj all_lines
+  val from_def = Define [ANTIQUOTE tm]
+  (* define decoding from cv type, i.e. "to function" *)
+  val tyvar_decoders = mapi (fn i => fn ty =>
+    mk_var("t" ^ int_to_string i,mk_type("fun",[cvSyntax.cv,ty]))) tyvars
+  val to_names = names |>
+    map (fn (fname,ty) =>
+      make_stem ("to_" ^ fname) tyvar_decoders (mk_funtype [cvSyntax.cv] ty))
+  val lookups =
+    map (fn tm => (tm |> type_of |> dest_fun_type |> snd, tm)) (to_names @ tyvar_decoders)
+  val cv_var = mk_var("v",cvSyntax.cv)
+  (*
+  val to_f = el 2 to_names
+  *)
+  fun to_lines to_f = let
+    val conses = to_f |> type_of |> dest_type |> snd |> el 2 |> constructors_of
+    val lhs_tm = mk_comb(to_f,cv_var)
+    (*
+      val i = 0
+      val cons_tm = el 1 conses
+    *)
+    fun to_line i cons_tm = let
+      val (tys,_) = dest_fun_types (type_of cons_tm)
+      val pat_args = mapi (fn i => fn ty => mk_var("v" ^ int_to_string i, ty)) tys
+      val pat = list_mk_comb(cons_tm,pat_args)
+      fun get_args v [] = []
+        | get_args v [x] = [(x,v)]
+        | get_args v (x::xs) =
+            (x,cvSyntax.mk_cv_fst v) :: get_args (cvSyntax.mk_cv_snd v) xs
+      val special = (listSyntax.is_cons pat orelse pairSyntax.is_pair pat)
+      val init_var = (if special then cv_var else cvSyntax.mk_cv_snd cv_var)
+      val args = get_args init_var tys
+      fun process_arg (ty,v) =
+        case alookup ty lookups of
+          SOME tm => mk_comb(tm,v)
+        | NONE => mk_comb(to_for ty,v)
+      val xs = map process_arg args
+      fun lemmas_for_arg (ty,v) =
+        case alookup ty lookups of
+          SOME tm => []
+        | NONE => [from_to_for ty]
+      val ys = map lemmas_for_arg args |> flatten
+      val build = list_mk_comb (cons_tm,xs)
+      val tag_num = cvSyntax.mk_cv_num(numSyntax.term_of_int i)
+      val c2b = c2b_def |> SPEC_ALL |> concl |> dest_eq |> fst |> rator
+      val none_num = optionSyntax.mk_none(num_ty)
+      val test = if null tys then mk_eq(cv_var,tag_num) else
+                   list_mk_comb(cv_has_shape_tm,
+                     [listSyntax.mk_list(
+                       (if special then [] else [optionSyntax.mk_some(tag_num |> rand)])
+                      @ replicate (length tys - 1) none_num,
+                      type_of none_num),
+                      cv_var])
+      in (ys,(test,build)) end
+    val lemmas_lines = mapi to_line conses
+    val lemmas = map fst lemmas_lines |> flatten
+    val lines = map snd lemmas_lines
+    fun partition p [] = ([],[])
+      | partition p (x::xs) =
+        let val (xs1,ys1) = partition p xs
+        in if p x then (x::xs1,ys1) else (xs1,x::ys1) end
+    val common_vars = cv_var :: tyvar_decoders
+    fun every p [] = true
+      | every p (x::xs) = (p x andalso every p xs)
+    fun exists p [] = false
+      | exists p (x::xs) = (p x orelse exists p xs)
+    fun subset xs ys = every (fn x => exists (aconv x) ys) xs
+    val (lines1,lines2) =
+      partition (fn (x,tm) => not (subset (free_vars tm) common_vars)) lines
+    val lines = lines1 @ lines2
+    fun mk_rhs [] = fail()
+      | mk_rhs [(t,x)] = if null lines2 then mk_cond(t,x,mk_arb(type_of x)) else x
+      | mk_rhs ((t,x)::xs) = mk_cond(t,x,mk_rhs xs)
+    in (mk_eq(lhs_tm,mk_rhs lines),lemmas) end
+  val (all_lines,lemmas1) = unzip (map to_lines to_names)
+  val lemmas = lemmas1 |> flatten
+  val tm = list_mk_conj all_lines
+  val cv_size =
+    cv_size_def |> CONJUNCTS |> hd |> SPEC_ALL |> concl |> dest_eq |> fst |> rator
+  val args = pairSyntax.list_mk_pair (tyvar_decoders @ [cv_var])
+  val size_tm = pairSyntax.mk_pabs(args, mk_comb(cv_size,cv_var))
+  fun mk_measure_input_ty [] = type_of args
+    | mk_measure_input_ty [x] = type_of args
+    | mk_measure_input_ty (x::xs) =
+        mk_sum_type (type_of args) (mk_measure_input_ty xs)
+  val measure_ty = mk_measure_input_ty all_lines
+  val measure_var = mk_var("x",measure_ty)
+  fun mk_cases [] = fail()
+    | mk_cases [x] = size_tm
+    | mk_cases (x::xs) =
+       mk_abs (mk_var("x",mk_measure_input_ty (x::xs)),
+         (mk_sum_case
+           (mk_var("x",mk_measure_input_ty (x::xs)))
+           size_tm (mk_cases xs)))
+  val measure_tm = mk_cases all_lines
+  val full_measure_tm = ISPEC measure_tm prim_recTheory.WF_measure |> concl |> rand
+  val to_def_name = (to_names |> hd |> repeat rator |> dest_var |> fst)
+  val to_def = tDefine to_def_name [ANTIQUOTE tm]
+    (WF_REL_TAC [ANTIQUOTE full_measure_tm]
+     \\ rewrite_tac [cv_has_shape_expand]
+     \\ rpt strip_tac \\ gvs [cv_size_def])
+  (* from from_to theorems *)
+  val assums =
+    map2 (fn f => fn t => ISPECL [f,t] from_to_def |> concl |> dest_eq |> fst)
+     (tyvar_encoders) (tyvar_decoders)
+  val assum = if null assums then T else list_mk_conj assums
+  fun term_all_distinct [] = []
+    | term_all_distinct (x::xs) = x :: term_all_distinct (filter (fn c => not (aconv c x)) xs)
+  val to_cs = to_def |> CONJUNCTS |> map (rator o fst o dest_eq o concl o SPEC_ALL)
+  val from_cs = from_def |> CONJUNCTS |> map (rator o fst o dest_eq o concl o SPEC_ALL)
+                                      |> term_all_distinct
+  val goals =
+    map2 (fn f => fn t =>
+      let
+        val ty = f |> type_of |> dest_fun_type |> fst
+        val v = mk_var("v",ty)
+      in mk_abs(v,mk_eq(mk_comb(t,mk_comb(f,v)),v)) end) from_cs to_cs
+  val lemma = ISPECL goals ind |> CONV_RULE (DEPTH_CONV BETA_CONV)
+  val main_goal = lemma |> concl |> dest_imp |> snd
+  val the_goal = mk_imp(assum,main_goal)
+  (*
+    set_goal([],the_goal)
+  *)
+  val from_to_thm = auto_prove "from_to_thm" (the_goal,
+    strip_tac
+    \\ match_mp_tac lemma
+    \\ rpt conj_tac
+    \\ rpt gen_tac
+    \\ rpt disch_tac
+    \\ once_rewrite_tac [from_def]
+    \\ once_rewrite_tac [to_def]
+    \\ rewrite_tac [cv_has_shape_def,cv_fst_def,cv_snd_def]
+    \\ EVERY (map assume_tac lemmas)
+    \\ fs [from_to_def])
+  val from_to_thms =
+    from_to_thm |> REWRITE_RULE [GSYM from_to_def]
+                |> UNDISCH_ALL |> CONJUNCTS
+                |> (fn xs => List.take(xs,mutrec_count))
+                |> map DISCH_ALL
+  (* simplify from_def *)
+  val froms = from_def |> CONJUNCTS |> map SPEC_ALL
+  val pick = (rator o fst o dest_eq o concl)
+  val from_heads = froms |> map pick |> term_all_distinct
+  val from_eqs = map (fn h => LIST_CONJ (filter (fn tm => aconv (pick tm) h) froms))
+                     (List.drop(from_heads,mutrec_count))
+                   |> map (DefnBase.one_line_ify NONE)
+  fun simp_from_eq from_eq = let
+    val v = from_eq |> concl |> dest_eq |> fst |> rand
+    val tyname = v |> type_of |> dest_type |> fst
+    in if tyname = "prod" then
+         from_eq |> CONV_RULE (RAND_CONV $ REWR_CONV get_from_pair)
+                 |> GEN v |> SIMP_RULE std_ss [GSYM FUN_EQ_THM,SF ETA_ss]
+       else if tyname = "option" then
+         from_eq |> CONV_RULE (RAND_CONV $ REWR_CONV get_from_option)
+                 |> GEN v |> SIMP_RULE std_ss [GSYM FUN_EQ_THM,SF ETA_ss]
+       else if tyname = "sum" then
+         from_eq |> CONV_RULE (RAND_CONV $ REWR_CONV get_from_sum)
+                 |> GEN v |> SIMP_RULE std_ss [GSYM FUN_EQ_THM,SF ETA_ss]
+       else if tyname = "list" then
+         let
+           val tm0 = from_eq |> concl |> dest_eq |> fst |> rator
+           val tm1 = from_eq |> concl |> rand |> rand |> dest_abs |> snd
+                             |> dest_abs |> snd |> rator |> rand |> rator
+           val tm2 = from_list_def |> CONJUNCT1 |> ISPEC tm1 |> concl
+                             |> dest_eq |> fst |> rator
+           val list_goal = mk_eq(tm0,tm2)
+           val res = auto_prove "simp_from_eq_list"
+                                (list_goal,
+                                 rewrite_tac [FUN_EQ_THM]
+                                 \\ Induct
+                                 \\ once_rewrite_tac [from_list_def,from_eq] \\ fs [])
+         in res end
+       else failwith ("simp_from_eq can't do: " ^ tyname) end
+  val from_simps = map simp_from_eq from_eqs
+  val from_def = map (fn h => LIST_CONJ (filter (fn tm => aconv (pick tm) h) froms))
+                     (List.take(from_heads,mutrec_count))
+                   |> LIST_CONJ |> REWRITE_RULE from_simps
+  (* simplify to_def *)
+  val ts = to_def |> CONJUNCTS
+  val ts0 = List.take(ts,mutrec_count)
+  val ts1 = List.drop(ts,mutrec_count) |> map SPEC_ALL
+  (*
+  val to_eq = el 1 ts1
+  *)
+  fun simp_one to_eq = let
+    val ty = to_eq |> concl |> dest_eq |> snd |> type_of
+    val tyname = dest_type ty |> fst
+    in if tyname = "option" then
+         to_eq |> REWRITE_RULE [get_to_option] |> GEN cv_var
+               |> SIMP_RULE std_ss [GSYM FUN_EQ_THM]
+               |> CONV_RULE (DEPTH_CONV ETA_CONV)
+       else if tyname = "sum" then
+         to_eq |> REWRITE_RULE [get_to_sum] |> GEN cv_var
+               |> SIMP_RULE std_ss [GSYM FUN_EQ_THM]
+               |> CONV_RULE (DEPTH_CONV ETA_CONV)
+       else if tyname = "prod" then
+         to_eq |> REWRITE_RULE [get_to_pair] |> GEN cv_var
+               |> SIMP_RULE std_ss [GSYM FUN_EQ_THM]
+               |> CONV_RULE (DEPTH_CONV ETA_CONV)
+       else if tyname = "list" then
+         let
+           val tm1 = to_eq |> concl |> dest_eq |> fst |> rator
+           val tm2 = to_eq |> concl |> dest_eq |> snd |> rator
+                           |> rand |> rator |> rand |> rator
+           val tm3 = to_list_def |> CONJUNCT1 |> ISPEC tm2 |> SPEC_ALL
+                                 |> concl |> dest_eq |> fst |> rator
+           val list_goal = mk_eq(tm1,tm3)
+           val res = auto_prove "to_list_eq"
+                        (list_goal,
+                         rewrite_tac [FUN_EQ_THM]
+                         \\ Induct
+                         \\ once_rewrite_tac [to_eq]
+                         \\ asm_rewrite_tac [to_list_def,cv_has_shape_def,
+                                             cv_fst_def,cv_snd_def])
+         in res end
+       else failwith ("don't know: " ^ tyname) end
+  val to_simps = map simp_one ts1
+  val to_def = ts0 |> map SPEC_ALL |> LIST_CONJ |> REWRITE_RULE to_simps
+  (* save all results *)
+  val th1 = save_thm("from_" ^ first_name ^ "_def[compute]", from_def)
+  val th2 = save_thm("to_" ^ first_name ^ "_def[compute]", to_def)
+  fun save_from_to_thms th = let
+    val to_name = th |> UNDISCH_ALL |> concl |> rand |> repeat rator |> dest_const |> fst
+    in save_thm("from_" ^ to_name ^ "_thm", th) end
+  val thms = List.map save_from_to_thms from_to_thms
+  in (from_def,to_def,from_to_thms) end
+
+(* tests *)
+
+Datatype:
+  a = A1 (num list) (((a # b) list) list)
+    | A2 ((a + b) list) ;
+  b = B1
+    | B2
+    | B3 (c option) ;
+  c = C1
+    | C2 a 'aa 'bb
+End
+
+val ty = “:('d, 'c) b”
+val res = define_from_to ty
+
+Datatype:
+  tree = Leaf
+       | Branch ((tree list + tree) option list)
+End
+
+val ty = “:tree”
+val res = define_from_to ty
 
 val _ = export_theory();
